SystemFD/Metatheory/Progress.lean
@@ -5,7 +5,6 @@ import SystemFD.Judgment
 import SystemFD.Metatheory.Classification
 import SystemFD.Reduction
 
-
 inductive Neutral : Ctx Term -> Term -> Prop where
   | varNe : ¬ Γ.is_stable n
           -> Neutral Γ (#n)
@@ -43,17 +42,35 @@ theorem var_neutral_form : (#n).neutral_form = .some (n, []) := by simp_all
 
 theorem lift_stable {Γ : Ctx Term} {n : Nat} : (Ctx.is_stable Γ n) -> ((Ctx.is_stable Γ n) = true) := by simp_all;
 
-theorem refl_is_val : Γ ⊢ η : (A ~ B) -> Val Γ η -> η = refl! A ∧ A = B := by
-intros ηJ vη; induction vη;
-case _ => simp_all; sorry
+def DeclCtx (Γ : Ctx Term) : Prop := ∀ n, ¬ Γ.is_lam_bound n
+
+theorem refl_is_val : DeclCtx Γ -> Γ ⊢ η : (A ~ B)
+                    -> Val Γ η
+                    -> η = refl! A ∧ A = B := by
+
+intros dctx ηJ vη; induction vη;
+case _ Γ t n _ _ n_stable =>
+  have x_no_lam : ¬ Γ.is_lam_bound n := dctx n;
+  unfold Ctx.is_stable at n_stable;
+  unfold Frame.is_stable at n_stable;
+  split at n_stable;
+  any_goals (solve | simp_all)
+  case _ =>
+    unfold Ctx.is_lam_bound at x_no_lam; unfold Frame.is_lam_bound at x_no_lam;
+    split at x_no_lam;
+    any_goals (solve | simp_all)
+    case _ => simp_all; sorry
+
 case _ => cases ηJ
 case _ => cases ηJ
 case _ => cases ηJ; simp_all
 
 
-theorem invert_appk_val : Γ ⊢ t : (A -k> B) -> Val Γ t -> ∃ t', (.kind A :: Γ) ⊢ t' : B ∧ t = Λ[A] t' := by
-intros tJ vt; induction vt;
-case _ => simp_all;  sorry
+theorem invert_appk_val : Γ ⊢ t : (A -k> B)
+                       -> Val Γ t -> t.neutral_form = .none
+                       -> t = Λ[A] t' := by
+intros tJ vt tnotnormal; induction vt;
+case _ => simp_all
 case _ => cases tJ
 case _ => cases tJ
 case _ => cases tJ
@@ -62,59 +79,35 @@ case _ => cases tJ
 theorem unique_neutral_form : (Term.neutral_form t = .some (n, sp)) -> (Term.neutral_form t = .some (n', sp')) -> (n = n') := by
 intros tnf tnf';
 induction t using Term.neutral_form.induct;
-case _ => simp_all;
-case _ => simp_all;
-case _ => simp_all;
-case _ => simp_all;
-case _ => simp_all
+any_goals (solve | simp_all)
 
-theorem openm_no_stable : Term.is_openmethod Γ n = true -> ¬ Ctx.is_stable Γ n := by
-intros om; simp_all; split at om;
-case _ => unfold Frame.is_stable; simp_all
+theorem openm_no_stable {Γ : Ctx Term}{n : Nat} :
+  Frame.is_openm (Γ d@ n) = true -> ¬ (Frame.is_stable (Γ d@ n)) := by
+intros om; simp_all; unfold Frame.is_openm at om; split at om;
+case _ => unfold Frame.is_stable; simp_all;
 case _ => simp_all
 
 theorem stable_no_reduce : t.neutral_form = .some (n, sp) -> Γ.is_stable n = true -> ¬ ∃ t', Red Γ t t' := by
 intros tnf nstable x; cases x;
   case _ w h =>
-  simp_all; induction h;
-  case _ => simp_all
-  case _ => simp_all
-  case _ => simp_all
-  case _ => simp_all
-  case _ => simp_all
-  case _ => simp_all
-  case _ => simp_all
-  case _ => simp_all
-  case _ => simp_all
-  case _ => simp_all
-  case _ => simp_all
-  case _ => simp_all
-  case _ => simp_all
-  case _ => simp_all
-  case _ => simp_all
-  case _ om _ _ _ => sorry
-  case _ idx => sorry
+  simp_all; induction h generalizing n sp;
+  any_goals (solve | simp_all)
+  case _ Γ _ _ _ _ om _ _ nstable =>
+    simp_all; sorry
+  case _ hnf idx =>
+    unfold Frame.is_stable at nstable; symm at hnf;
+    have uniq := unique_neutral_form hnf tnf; subst uniq; rw [<-idx] at nstable; simp_all
   case _ f _ _ _ _ _ nosome =>
     simp_all; rw[Option.bind_eq_some] at tnf;
-    cases tnf; case _ h =>
+    cases tnf; case _ w h =>
       simp_all; have wfst := And.left (And.right h);
       have wsnd := And.right (And.right h);
+      have cc := @nosome n sp;
       sorry
-  case _ => simp_all
-  case _ => simp_all
-  case _ => simp_all
-  case _ => simp_all
-  case _ => simp_all
-  case _ => simp_all
-  case _ => simp_all
-  case _ => simp_all
-  case _ => simp_all
-  case _ => simp_all
-  case _ => simp_all
-  case _ => simp_all
-  case _ => simp_all
-  case _ => simp_all
-  case _ => simp_all
+  case _ ih =>
+    simp_all; rw [Option.bind_eq_some] at tnf;
+    cases tnf; case _ w h =>
+    have nih := And.left h; sorry
 
 theorem val_no_red : Val Γ t -> ¬ ∃ t', Red Γ t t' := by
 intros vt tred; induction vt;
@@ -125,195 +118,171 @@ case _ =>
 case _ => cases tred; case _ h =>
   cases h;
   case _ => simp_all
-case _ => cases tred; case _ h =>
-  cases h;
   case _ => simp_all
 case _ => cases tred; case _ h =>
   cases h;
+  case _ => simp_all
+  case _ => simp_all
+case _ => cases tred; case _ h =>
+  cases h;
+  case _ => simp_all
   case _ => simp_all
 
 @[simp]
 abbrev MaybeStep : (v : JudgmentVariant) -> (Γ : Ctx Term) -> (JudgmentArgs v) -> Prop
-| .prf => λ Γ => λ(t , _) => Neutral Γ t ∨ Val Γ t ∨ ∃ t', Red Γ t t'
+| .prf => λ Γ => λ(t , A) => (∃ K, Γ ⊢ K : .kind ∧ Γ ⊢ A : K) ->  Neutral Γ t ∨ Val Γ t ∨ ∃ t', Red Γ t t'
 | .wf  => λ _ => λ () => true
 
 theorem progress_lemma : Judgment v Γ ix -> MaybeStep v Γ ix := by
 intros j; induction j;
-case _ => simp_all
-case _ => simp_all
-case _ => simp_all
-case _ => simp_all
-case _ => simp_all
-case _ => simp_all
-case _ => simp_all
-case _ => simp_all
-case _ => simp_all
-case _ => simp_all
-
-case _ ih =>
-  simp_all; cases ih;
-  case _ h => sorry -- apply Or.inr (Or.inr Red.letterm);
-  case _ => sorry -- apply Or.inr (Or.inr Red.letterm);
-case _ =>
-  simp; sorry -- uses classification lemma?
-case _ => simp_all; sorry -- uses classification lemma?
-case _ => simp_all; sorry -- uses classification lemma?
-case _ ih _ =>
-  simp_all; cases ih;
-  case _ => sorry
-  case _ h =>
-  cases h;
-  case _ => sorry
-  case _ => sorry
+any_goals (solve | simp_all)
+all_goals (intro h)
+case _ Γ A t b _ _ _ _ _ _ _ ih _ =>
+  simp_all;
+  generalize tl' : [b β[ t ]] = t' at *; symm at tl';
+  have reds := @Red.letbeta Γ A t b; rw [<-tl']  at reds;
+  have ereds : ∃ t', Red Γ (.letterm A t b) t' := Exists.intro t' reds;
+  apply Or.inr (Or.inr ereds);
+case _ => cases h; case _ w h => cases h.2;
+ -- VAR
+case _ => sorry
+case _ => cases h; case _ h => cases h.2
+case _ => cases h; case _ h => cases h.2; sorry
+case _ => cases h; case _ h => cases h.2; sorry -- uses classification lemma
 case _ => simp_all; sorry -- uses classification lemma
 case _ => simp_all; sorry -- uses classification lemma
-case _ => simp_all; sorry -- uses classification lemma
-case _ p _ s _ b _ _ c _ _ _ _ phead _ hmatch prefixmatch _ _ pih sih _ _ _ _ =>
-  simp_all; cases pih;
-  case _ ph => sorry
-  case _ ph =>
-    cases ph;
-    case _ ph =>
-      cases sih;
-      case _ h => apply Or.inl (Neutral.iteNe h)
-      case _ h =>
-      cases h;
-      case _ h =>
-        cases hmatch;
-        case refl x _ =>
-          cases x;
-          case _ =>
-          cases phead;
-          case _ pnf pJ => sorry
-        case _ x => sorry
-        case _ x => sorry
-      case _ h =>
-      cases h; case _ w h =>
-      generalize tlp' : List.map (Term.ite p · b c) w = tl' at *; symm at tlp';
-      have t' := Red.ite_congr h tlp';
-      apply Or.inr (Or.inr (Exists.intro tl' t'))
-    case _ ph =>
-    cases ph; case _ ts preds =>
-    cases phead; case _ w pctor =>
-      simp_all; have pctorstable := Frame.is_ctor_implies_is_stable (And.right pctor);
-      have pnf := And.left pctor; symm at pnf;
-      have pnoreds := stable_no_reduce pnf pctorstable;
-      have preds := Exists.intro ts preds; simp_all;
-case _ => sorry
-case _ => sorry
-case _ => sorry
-case _ => sorry
-case _ => sorry
-case _ ih =>  simp_all; sorry
 
-case _ => simp_all; sorry
-case _ => simp_all; sorry
-case _ => simp_all; sorry
-case _ => simp_all; sorry
-case _ => simp_all; sorry
-case _ => simp_all; sorry
-case _ => simp_all; sorry
-case _ => simp_all; sorry
-case _ => simp_all; sorry
+-- ITE
+case _ Γ p _ s _ b _ _ c _ _ _ _ phead _ hmatch prefixmatch _ _ pih sih _ _ _ _ =>
+  simp at pih;
+  sorry
+  -- simp_all; cases pih;
+  -- case _ ph =>
+  --   cases phead; sorry
+  -- case _ ph =>
+  --   cases ph;
+  --   case _ ph =>
+  --     cases sih;
+  --     case _ h => apply Or.inl (Neutral.iteNe h)
+  --     case _ h =>
+  --     cases h;
+  --     case _ h =>
+  --       cases hmatch;
+  --       case refl x _ =>
+  --         cases x;
+  --         case _ =>
+  --         cases phead;
+  --         case _ pnf pJ => sorry
+  --       case _ x => sorry
+  --       case _ x => sorry
+  --     case _ h =>
+  --     cases h; case _ w h =>
+  --     generalize tlp' : List.map (Term.ite p · b c) w = tl' at *; symm at tlp';
+  --     have t' := Red.ite_congr h tlp';
+  --     apply Or.inr (Or.inr (Exists.intro tl' t'))
+  --   case _ ph =>
+  --   cases ph; case _ ts preds =>
+  --   cases phead; case _ w pctor =>
+  --     simp_all; have pctorstable := Frame.is_ctor_implies_is_stable (And.right pctor);
+  --     have pnf := And.left pctor; symm at pnf;
+  --     have pnoreds := stable_no_reduce pnf pctorstable;
+  --     have preds := Exists.intro ts preds; simp_all;
+-- GUARD
+case _ => sorry
 
--- theorem progress_νT :
---     (Γ ⊢ A : ★) -> (Γ ⊢ t : A)
--- --------------------------------------
---   -> Val Γ t ∨ ∃ t', Red Γ t t' := by
--- intros Astar typingJ;
--- cases typingJ;
--- case _ => cases Astar
--- case _ => cases Astar
--- case _ => cases Astar
--- case _ => cases Astar
--- case _ => cases Astar
--- case _ => cases Astar
--- case _ => cases Astar
--- case _ => cases Astar
--- case _ n _  aTy =>
---   unfold Frame.get_type at aTy;
---   cases Γ d@ n;
---   case _ => sorry
---   case _ => sorry
---   case _ => sorry
---   case _ => sorry
---   case _ => sorry
---   case _ => sorry
---   case _ => sorry
---   case _ => sorry
---   case _ => sorry
---   case _ => sorry
---   -- match Γ d@ n with
---   -- | .empty =>  at aTy; simp at aTy;  sorry
---   -- | .kind _ => sorry
---   -- | .type _ => sorry
---   -- | .datatype _ => sorry
---   -- | .ctor _ => sorry
---   -- | .opent _ => sorry
---   -- | .openm _ => sorry
---   -- | .insttype _ => sorry
---   -- | .inst _ _ => sorry
---   -- | .term _ _ => sorry
+case _ Γ A t _ _ _ _ _ _ _  =>
+  simp_all; have vlam : Val Γ (`λ[A] t) :=  (@Val.lam Γ A t); apply Or.inr (Or.inl vlam);
+case _ => sorry
+case _ Γ A t _ _ _ _ _ _ _ =>
+    simp_all; have vlam : Val Γ (Λ[A] t) :=  (@Val.lamt Γ A t); apply Or.inr (Or.inl vlam);
+case _ => sorry
+case _ ih => sorry
 
--- case _ => cases Astar
--- case _ => sorry -- proof by classification lemma
--- case _ => cases Astar
--- case _ f _ _ aty arrk => sorry -- proof by classification lemma
--- case _ => cases Astar
--- case _ => sorry
--- -- case _ p _ s _ i _ _ _ e _ _ pJ sJ Rstar cJ _ _ _ _ eJ => sorry
---   -- cases progress_νT Rstar sJ;
---   -- case _ νs => apply Or.inl (.iteNe νs)
---   -- case _ h => cases h; case _ w r =>
---   --   generalize tlp' : List.map (Term.ite p · i e) w = tl' at *; symm at tlp';
---   --   have t' := Red.ite_congr r tlp';
---   --   apply (Or.inr (Exists.intro tl' t'))
--- case _ p _ s _ t _ pJ sJ Rstar _ _ _ _ => sorry
---   -- cases progress_νT Rstar sJ;
---   -- case _ νs => apply (Or.inl (.guardNe νs))
---   -- case _ h => cases h; case _ w r =>
---   -- generalize tlp' : List.map (Term.guard p · t) w = tl' at *; symm at tlp';
---   -- have t' := Red.guard_congr r tlp';
---   -- apply (Or.inr (Exists.intro tl' t'))
--- case _ => apply Or.inl .lam
--- case _ f A B a fJ aJ _ => sorry
---   -- have arrStar : (Γ ⊢ (A -t> B) : ★) := .arrow sorry sorry;
---   -- cases (progress_νT arrStar fJ);
---   -- case _ h => apply Or.inl (.appNe h)
---   -- case _ h => cases h; case _ w r =>
---   -- generalize tlp' : List.map ( · `@ a) w = tl' at *; symm at tlp';
---   -- have t' := Red.app_congr r tlp';
---   -- apply (Or.inr (Exists.intro tl' t'))
--- case _ => apply Or.inl .lamt
--- case _ f A B a fJ aJ _ => sorry
--- --   have allStar : (Γ ⊢ (∀[A] B) : ★) := .allt sorry sorry sorry;
--- --   cases (progress_νT allStar fJ);
--- --   case _ h => apply Or.inl (.apptNe h)
--- --   case _ h => cases h; case _ w r =>
--- --   generalize tlp' : List.map ( · `@t a) w = tl' at *; symm at tlp';
--- --   have t' := Red.appt_congr r tlp';
--- --   apply (Or.inr (Exists.intro tl' t'))
--- case _ t B η tJ ηJ => sorry
---   -- have eqStar : (Γ ⊢ (B ~ A) : ★) := .eq sorry Astar;
---   -- cases (progress_νT eqStar  ηJ);
---   -- case _ h => apply (Or.inl (.castNe h))
---   -- case _ h => cases h; case _ w r =>
---   -- generalize tlp' : List.map (t ▹ ·) w = tl' at *; symm at tlp';
---   -- have t' := Red.cast_congr r tlp';
---   -- apply (Or.inr (Exists.intro tl' t'))
--- case _ => apply Or.inl .refl
--- case _ η A B ηJ => sorry
---   -- have eqStar : (Γ ⊢ (A ~ B) : ★) := flip_eq Astar;
---   -- cases progress_νT eqStar ηJ;
---   -- case _ h => apply Or.inl (.symNe h)
---   -- case _ h => cases h; case _ w r =>
---   -- generalize tlp' : List.map (sym! ·) w = tl' at *; symm at tlp';
---   -- have t' := Red.sym_congr r tlp';
---   -- apply (Or.inr (Exists.intro tl' t'))
--- case _ => sorry
--- case _ => sorry
--- case _ => sorry
--- case _ => sorry
--- case _ => sorry
--- case _ => sorry
--- case _ => sorry
+case _ => sorry
+case _ => sorry
+case _ => sorry
+case _ => sorry
+case _ => sorry
+case _ => sorry
+case _ => sorry
+case _ => sorry
+case _ => sorry
+
+
+@[simp]
+abbrev StepOrVal : (v : JudgmentVariant) -> (Γ : Ctx Term) -> (JudgmentArgs v) -> Prop
+| .prf => λ Γ => λ(t , A) => DeclCtx Γ -> (∃ K, Γ ⊢ K : .kind ∧ Γ ⊢ A : K) -> Val Γ t ∨ ∃ t', Red Γ t t'
+| .wf  => λ _ => λ () => true
+
+
+theorem progress :
+    Judgment v Γ ix
+--------------------------------------
+  -> StepOrVal v Γ ix := by
+intros j; induction j;
+any_goals (solve | simp_all)
+all_goals (intro dctx h)
+case _ Γ A t b _ _ _ _ _ _ _ ih _ =>
+  simp_all;
+  generalize tl' : [b β[ t ]] = t' at *; symm at tl';
+  have reds := @Red.letbeta Γ A t b; rw [<-tl']  at reds;
+  have ereds : ∃ t', Red Γ (.letterm A t b) t' := Exists.intro t' reds;
+  apply Or.inr ereds;
+
+case _ => cases h; case _ h => cases h.2;
+case var Γ x _ _ xTy ih =>
+  simp at ih; have x_no_lam := dctx x;
+  unfold Ctx.is_lam_bound at x_no_lam;
+  unfold Frame.is_lam_bound at x_no_lam;
+  unfold Frame.get_type at xTy; simp at xTy;
+  split at xTy;
+  any_goals (solve | simp_all)
+  case _ =>  -- classification lemma
+    sorry
+  case _ f t x_is_ctor =>
+    have xx : Frame.is_stable (Γ d@ x) := by unfold Frame.is_stable; rw[x_is_ctor];
+    have hh : (#x).neutral_form = .some (x, []) := var_neutral_form;
+    apply Or.inl (Val.app hh xx)
+  case _ =>    -- classification lemma
+    injection xTy with teqT; symm at teqT; subst teqT; cases h; case _ h =>
+    sorry
+  case _ x_is_openm =>  -- steps inst
+    have nf  := @var_neutral_form x; symm at nf;
+    have om : (Γ d@ x).is_openm := by unfold Frame.is_openm; rw [x_is_openm];
+    generalize isp : instance_indices' Γ 0 x [] = ιs at *; symm at isp;
+    generalize instsp : get_instances Γ ιs = insts at *; symm at instsp;
+    generalize instsp' : List.map (·.apply_spine []) insts = insts' at *; symm at instsp';
+    apply Or.inr (Exists.intro insts' (Red.inst nf om isp instsp instsp'))
+  case _ x_is_insttype =>  -- value
+    have xx : Frame.is_stable (Γ d@ x) := by unfold Frame.is_stable; rw[x_is_insttype];
+    have hh : (#x).neutral_form = .some (x, []) := var_neutral_form;
+    apply Or.inl (Val.app hh xx)
+  case _ A t x_frame =>  -- steps letterm
+    have nf : .some (x, []) = (#x).neutral_form := var_neutral_form;
+    have x_is_term : .term A t = Γ d@ x := by symm at x_frame; apply x_frame
+    generalize tlp : [t.apply_spine []] = t' at *; symm at tlp;
+    have etl' : ∃ t', Red Γ (#x) t' := Exists.intro ([t.apply_spine []]) (Red.letterm nf x_is_term);
+    apply Or.inr etl'
+
+case _ => cases h; case _ h => cases h.2
+case _ => cases h; case _ h => cases h.2; cases h.1;
+
+case _ => cases h; case _ h => cases h.2; cases h.1
+case _ =>  cases h; case _ h => sorry
+case _ => cases h; case _ h => cases h.2; cases h.1
+case ite => sorry
+case guard => sorry
+case _ _ A t _ _ _ _ _ _ _ => apply Or.inl Val.lam
+case _ => sorry
+case _ _ A t _ _ _ _ _ _ _ => apply Or.inl Val.lamt
+case _ => sorry
+case _ => sorry
+case _ => apply Or.inl Val.refl
+case _ Γ η _ _ _ _ => sorry
+case _ => sorry
+case _ => sorry -- cases h; case _ h => cases h.2; cases h.1
+case _ => cases h; case _ h => cases h.2; cases h.1; sorry
+case _ => sorry
+case _ => sorry
+case _ => cases h; case _ h => cases h.2; cases h.1; sorry
+case _ => sorry
