SystemFD/Examples/Boolean.lean
@@ -104,9 +104,9 @@ def EqBoolCtx : Ctx Term := [
 ]
 
 #eval wf_ctx EqBoolCtx
-#eval infer_type EqBoolCtx (#3 `@t #7 `@ (#2 `@t #7 `@ refl! #7) `@ #5 `@ #5) -- some `7
+#eval infer_type EqBoolCtx (#3 `@t #7 `@ (#2 `@t #7 `@ refl! #7) `@ #5 `@ #5) -- some 7
 
 -- == [Bool] (EqBool[Bool] refl) True True ⟶★ True
-#eval eval_ctx_loop EqBoolCtx (#3 `@t #7 `@ (#2 `@t #7 `@ refl! #7) `@ #5 `@ #5)
+#eval eval_ctx_loop EqBoolCtx (#3 `@t #7 `@ (#2 `@t #7 `@ refl! #7) `@ #5 `@ #5) -- some 5
 -- == [Bool] (EqBool[Bool] refl) True False ⟶★ False
-#eval eval_ctx_loop EqBoolCtx (#3 `@t #7 `@ (#2 `@t #7 `@ refl! #7) `@ #5 `@ #6)
+#eval eval_ctx_loop EqBoolCtx (#3 `@t #7 `@ (#2 `@t #7 `@ refl! #7) `@ #5 `@ #6) -- some 6
